Qsort/Monadic/Simp.lean
@@ -3,3 +3,7 @@ import Lean.Meta.Tactic.Simp
 register_simp_attr sort
 
 register_simp_attr spred
+
+register_simp_attr lists
+
+register_simp_attr arith
